wip: proving the last subgoal for the epoch correctness.

refinements/EpochInv.v
@@ -81,6 +81,106 @@ Section Processor.
   Definition D2R := D2R addrSize dataBytes rfIdx.
   Definition R2E := R2E addrSize dataBytes rfIdx.
 
+  Record EpochPc := { pPc : word addrSize;
+                      pPredPc : word addrSize;
+                      pDecEpoch : option bool;
+                      pExeEpoch : bool }.
+
+  Definition f2iToEpochPc (f2ie: type (Struct F2I)) :=
+    {| pPc := f2ie Fin.F1 Fin.F1;
+       pPredPc := f2ie Fin.F1 (Fin.FS Fin.F1);
+       pDecEpoch := Some (f2ie Fin.F1 (Fin.FS (Fin.FS Fin.F1)));
+       pExeEpoch := f2ie Fin.F1 (Fin.FS (Fin.FS (Fin.FS Fin.F1))) |}.
+
+  Definition i2dToEpochPc (i2de: type (Struct I2D)) :=
+    {| pPc := i2de Fin.F1 Fin.F1;
+       pPredPc := i2de Fin.F1 (Fin.FS Fin.F1);
+       pDecEpoch := Some (i2de Fin.F1 (Fin.FS (Fin.FS Fin.F1)));
+       pExeEpoch := i2de Fin.F1 (Fin.FS (Fin.FS (Fin.FS Fin.F1))) |}.
+
+  Definition d2rToEpochPc (d2re: type (Struct D2R)) :=
+    {| pPc := d2re Fin.F1;
+       pPredPc := d2re (Fin.FS Fin.F1);
+       pDecEpoch := None;
+       pExeEpoch := d2re (Fin.FS (Fin.FS (Fin.FS Fin.F1))) |}.
+
+  Definition r2eToEpochPc (r2ee: type (Struct R2E)) :=
+    {| pPc := r2ee Fin.F1;
+       pPredPc := r2ee (Fin.FS Fin.F1);
+       pDecEpoch := None;
+       pExeEpoch := r2ee (Fin.FS (Fin.FS (Fin.FS (Fin.FS (Fin.FS Fin.F1))))) |}.
+
+  (* NOTE: head is the oldest *)
+  Definition epochPcFidre
+             (f2iv: list (type (Struct F2I))) (i2dv: list (type (Struct I2D)))
+             (d2rv: list (type (Struct D2R))) (r2ev: list (type (Struct R2E))) :=
+    ((map r2eToEpochPc r2ev)
+       ++ (map d2rToEpochPc d2rv)
+       ++ (map i2dToEpochPc i2dv)
+       ++ (map f2iToEpochPc f2iv))%list.
+
+  Definition epochPcDre
+             (d2rv: list (type (Struct D2R))) (r2ev: list (type (Struct R2E))) :=
+    ((map r2eToEpochPc r2ev) ++ (map d2rToEpochPc d2rv))%list.
+
+  (** [pcChainFromPc] and [pcChainFromDec] describe invariants
+   * when there are no redirections, saying that pc/predPc pairs generate
+   * a chain (started from either [pc] or [decRedir]) throughout the fifos.
+   *)
+  Definition decEpochMatches (decEpoch: bool) (pDecEpoch: option bool) :=
+    match pDecEpoch with
+    | Some pde => eqb decEpoch pde
+    | None => true
+    end.
+
+  (* NOTE: head should be the youngest! *)
+  Fixpoint pcChainDecExe (pcv: fullType type (SyntaxKind (Bit addrSize)))
+           (decEpochv exeEpochv: fullType type (SyntaxKind Bool))
+           (eps: list EpochPc) :=
+    match eps with
+    | nil => True
+    | ep :: eps' =>
+      if (decEpochMatches decEpochv (pDecEpoch ep))
+           && (eqb exeEpochv (pExeEpoch ep))
+      then pcv = pPredPc ep /\ pcChainDecExe (pPc ep) decEpochv exeEpochv eps'
+      else True
+    end.
+  
+  Definition pcChainFromPc (pcv: fullType type (SyntaxKind (Bit addrSize)))
+             (decEpochv exeEpochv: fullType type (SyntaxKind Bool))
+             (f2iv: list (type (Struct F2I))) (i2dv: list (type (Struct I2D)))
+             (d2rv: list (type (Struct D2R))) (r2ev: list (type (Struct R2E))) :=
+    pcChainDecExe pcv decEpochv exeEpochv (List.rev (epochPcFidre f2iv i2dv d2rv r2ev)).
+
+  (* NOTE: head should be the youngest! *)
+  Fixpoint pcChainExe (pcv: fullType type (SyntaxKind (Bit addrSize)))
+           (exeEpochv: fullType type (SyntaxKind Bool))
+           (eps: list EpochPc) :=
+    match eps with
+    | nil => True
+    | ep :: eps' =>
+      if eqb exeEpochv (pExeEpoch ep)
+      then pcv = pPredPc ep /\ pcChainExe (pPc ep) exeEpochv eps'
+      else True
+    end.
+
+  Definition pcChainFromDec (pcv: fullType type (SyntaxKind (Bit addrSize)))
+             (exeEpochv: fullType type (SyntaxKind Bool))
+             (d2rv: list (type (Struct D2R))) (r2ev: list (type (Struct R2E))) :=
+    pcChainExe pcv exeEpochv (List.rev (epochPcDre d2rv r2ev)).
+
+  Definition getOldest
+             (f2i: list (type (Struct F2I))) (i2d: list (type (Struct I2D)))
+             (d2r: list (type (Struct D2R))) (r2e: list (type (Struct R2E))) :=
+    match epochPcFidre f2i i2d d2r r2e with
+    | nil => None
+    | hd :: _ => Some hd
+    end.
+
+  (** [consistentDecEpoch] and [consistentExeEpoch] describe invariants
+   * when a pc value is redirected from Decode or Execute, respectively,
+   * saying that all epoch values are same throughout the fifos.
+   *)
   Definition consistentDecEpochF2I (decEpoch: bool) (f2i: list (type (Struct F2I))) :=
     Forall (fun e : type (Struct F2I) => e Fin.F1 (Fin.FS (Fin.FS Fin.F1))
                                          = decEpoch) f2i.
@@ -115,7 +215,9 @@ Section Processor.
     consistentExeEpochD2R exeEpoch d2r /\ consistentExeEpochR2E exeEpoch r2e.
 
   Record epoch_invariant (o: RegsT) : Prop :=
-    { fetchEpochDv : fullType type (SyntaxKind Bool);
+    { pcv : fullType type (SyntaxKind (Bit addrSize));
+      Hpc: M.find "pc" o = Some (existT _ _ pcv);
+      fetchEpochDv : fullType type (SyntaxKind Bool);
       Hfed: M.find "fetchEpochD" o = Some (existT _ _ fetchEpochDv);
       fetchEpochEv : fullType type (SyntaxKind Bool);
       Hfee: M.find "fetchEpochE" o = Some (existT _ _ fetchEpochEv);
@@ -149,7 +251,22 @@ Section Processor.
       HdrSpec: decRedirv Fin.F1 = true ->
                consistentDecEpoch (negb decEpochv) f2iv i2dv;
       HerSpec: exeRedirv Fin.F1 = true ->
-               consistentExeEpoch (negb exeEpochv) f2iv i2dv d2rv r2ev
+               consistentExeEpoch (negb exeEpochv) f2iv i2dv d2rv r2ev;
+
+      (** Invariants with no redirections, about pc/predPc chain *)
+      Hchain1: decRedirv Fin.F1 = false ->
+               exeRedirv Fin.F1 = false ->
+               pcChainFromPc pcv decEpochv exeEpochv f2iv i2dv d2rv r2ev;
+      Hchain2: decRedirv Fin.F1 = true ->
+               exeRedirv Fin.F1 = false ->
+               pcChainFromDec (decRedirv (Fin.FS Fin.F1) (Fin.FS Fin.F1)) exeEpochv d2rv r2ev;
+
+      (** An invariant about exeEpoch *)
+      HeeSpec3: match getOldest f2iv i2dv d2rv r2ev with
+                | Some ep => pExeEpoch ep = exeEpochv ->
+                             consistentExeEpoch exeEpochv f2iv i2dv d2rv r2ev
+                | None => True
+                end
     }.
 
   Local Notation "'_STRUCT_'" := (fun i : Fin.t _ => _).
@@ -158,11 +275,18 @@ Section Processor.
   Lemma fidreComb_epoch_invariant_ok:
     forall o, reachable o fidreComb -> epoch_invariant o.
   Proof.
-    (* intros; apply stepInv with (m:= fidreComb); auto; *)
-    (*   [econstructor; *)
-    (*    try (findReify; (reflexivity || eassumption); fail); *)
-    (*    auto; try (intros; inv H0)|]. *)
+    (* intros; apply stepInv with (m:= fidreComb); auto. *)
 
+    (* Focus 1. (* initial case *) *)
+    (* econstructor; *)
+    (*   try (findReify; (reflexivity || eassumption); fail); *)
+    (*   auto. *)
+    (* intros; inv H0. *)
+    (* intros; inv H0. *)
+    (* intros; vm_compute; auto. *)
+    (* intros; vm_compute; auto. *)
+
+    (* (* induction case *) *)
     (* clear H o; intros. *)
     (* apply step_implies_stepDet in H0; *)
     (*   [|kequiv|repeat (constructor || reflexivity)|reflexivity]. *)
